abstract fresh var generation

theories/Bigstep.v
@@ -3,78 +3,81 @@ From Coq Require Import FMaps FSets.
 From Haskelite Require Import Expr Common.
 Import ListNotations.
 
-Inductive eval_expr : nat -> heap -> var_set -> expr -> 
-                      heap -> expr -> nat -> Prop :=
-  | EvalWhnf : forall c G L w,
+Section FreshGen.
+Context {FG : FreshVarGen}.
+
+Inductive eval_expr : heap -> var_set -> expr -> 
+                      heap -> expr -> Prop :=
+  | EvalWhnf : forall G L w,
       whnf w ->
-      eval_expr c G L w G w c
+      eval_expr G L w G w
 
-  | EvalSat : forall c c1 c2 G L m e D O w,
+  | EvalSat : forall G L m e D O w,
       matching_arity m = Some 0 ->
-      eval_matching c G L [] m D (MRReturn e) c1 ->
-      eval_expr c1 D L e O w c2 ->
-      eval_expr c G L (ELam m) O w c2
+      eval_matching G L [] m D (MRReturn e) ->
+      eval_expr D L e O w ->
+      eval_expr G L (ELam m) O w
 
-  | EvalVar : forall c c' G L y e D w,
+  | EvalVar : forall G L y e D w,
       heap_lookup G y = Some e ->
       ~ (In y L) ->
-      eval_expr c (heap_remove G y) (y :: L) e D w c' -> (* black-holing *)
-      eval_expr c G L (EVar y) (heap_update D y w) w c'
+      eval_expr (heap_remove G y) (y :: L) e D w -> (* black-holing *)
+      eval_expr G L (EVar y) (heap_update D y w) w
 
-  | EvalApp : forall c c1 c2 G L e1 e2 m D O w x,
-      eval_expr c G L e1 D (ELam m) c1 ->
+  | EvalApp : forall G L e1 e2 m D O w x,
+      eval_expr G L e1 D (ELam m) ->
       e2 = EVar x ->
       (* e2 should be a variable *)
-      eval_expr c1 D L (ELam (MSupply (EVar x) m)) O w c2 ->
-      eval_expr c G L (EApp e1 e2) O w c2
+      eval_expr D L (ELam (MSupply (EVar x) m)) O w ->
+      eval_expr G L (EApp e1 e2) O w
 
-with eval_matching : nat -> heap -> var_set -> list var -> matching -> 
-                     heap -> matching_result -> nat -> Prop :=
+with eval_matching : heap -> var_set -> list var -> matching -> 
+                     heap -> matching_result -> Prop :=
 
   (*eval_matching c G (update_locs St) A (MReturn e0) D (MRReturn (apply_args A e0)) c'*)
-  | EvalReturn : forall c G L A e,
-      eval_matching c G L A (MReturn e) G (MRReturn (apply_args A e)) c
+  | EvalReturn : forall G L A e,
+      eval_matching G L A (MReturn e) G (MRReturn (apply_args A e))
 
-  | EvalMatchFail : forall c G L,
-      eval_matching c G L [] MFail G MRFail c
+  | EvalMatchFail : forall G L,
+      eval_matching G L [] MFail G MRFail
 
-  | EvalArg : forall c c' G L A x m D u,
-      eval_matching c G L (x :: A) m D u c' ->
-      eval_matching c G L A (MSupply (EVar x) m) D u c'
+  | EvalArg : forall G L A x m D u,
+      eval_matching G L (x :: A) m D u ->
+      eval_matching G L A (MSupply (EVar x) m) D u
 
-  | EvalBindVar : forall c c' G L A x y m D u,
-      eval_matching c G L A (subst_matching m y x) D u c' ->
-      eval_matching c G L (y :: A) (MMatch (PVar x) m) D u c'
+  | EvalBindVar : forall G L A x y m D u,
+      eval_matching G L A (subst_matching m y x) D u ->
+      eval_matching G L (y :: A) (MMatch (PVar x) m) D u
 
-  | EvalConsMatch : forall c c1 c2 G L A x cp ps m args D O u,
-      eval_expr c G L (EVar x) D (ECons cp (map EVar args)) c1 ->
+  | EvalConsMatch : forall G L A x cp ps m args D O u,
+      eval_expr G L (EVar x) D (ECons cp (map EVar args)) ->
       length ps = length args ->
-      eval_matching c1 D L A (build_nested_matches args ps m) O u c2 ->
-      eval_matching c G L (x :: A) (MMatch (PCons cp ps) m) O u c2
+      eval_matching D L A (build_nested_matches args ps m) O u ->
+      eval_matching G L (x :: A) (MMatch (PCons cp ps) m) O u
 
-  | EvalConsFail : forall c c' G L A x cp cp' ps m args D,
-      eval_expr c G L (EVar x) D (ECons cp' args) c' ->
+  | EvalConsFail : forall G L A x cp cp' ps m args D,
+      eval_expr G L (EVar x) D (ECons cp' args) ->
       cp <> cp' ->
-      eval_matching c G L (x :: A) (MMatch (PCons cp ps) m) D MRFail c'
+      eval_matching G L (x :: A) (MMatch (PCons cp ps) m) D MRFail
 
-  | EvalAltLeft : forall c c' G L A m1 m2 e D,
-      eval_matching c G L A m1 D (MRReturn e) c' ->
-      eval_matching c G L A (MAlt m1 m2) D (MRReturn e) c'
+  | EvalAltLeft : forall G L A m1 m2 e D,
+      eval_matching G L A m1 D (MRReturn e) ->
+      eval_matching G L A (MAlt m1 m2) D (MRReturn e)
 
-  | EvalAltRight : forall c c1 c2 G L A m1 m2 D O u,
-      eval_matching c G L A m1 D MRFail c1 ->
-      eval_matching c1 D L A m2 O u c2 ->
-      eval_matching c G L A (MAlt m1 m2) O u c2
+  | EvalAltRight : forall G L A m1 m2 D O u,
+      eval_matching G L A m1 D MRFail ->
+      eval_matching D L A m2 O u ->
+      eval_matching G L A (MAlt m1 m2) O u
 
-  | EvalWhere : forall c G L A m binds D u ys renamed_binds renamed_m,
+  | EvalWhere : forall G L A m binds D u ys renamed_binds renamed_m,
       (* generate fresh variables using counter *)
-      ys = gen_n_fresh c (length binds) ->
+      ys = gen_fresh L (length binds) ->
       (* perform renaming *)
       renamed_binds = rename_bindings binds ys ->
       renamed_m = rename_matching m ys binds ->
       (* allocate renamed bindings and continue with incremented counter *)
-      eval_matching (c + length binds) (allocate_bindings G renamed_binds) L A renamed_m D u (c + length binds) ->
-      eval_matching c G L A (MWhere m binds) D u (c + length binds)
+      eval_matching (allocate_bindings G renamed_binds) L A renamed_m D u ->
+      eval_matching G L A (MWhere m binds) D u
 .
 
 
@@ -83,8 +86,8 @@ with eval_matching_ind_mutual := Induction for eval_matching Sort Prop.
 
 Combined Scheme eval_ind from eval_expr_ind_mutual, eval_matching_ind_mutual.
 
-Lemma eval_expr_produces_whnf : forall c G L e D w c',
-  eval_expr c G L e D w c' -> whnf w.
+Lemma eval_expr_produces_whnf : forall G L e D w,
+  eval_expr G L e D w -> whnf w.
 Proof.
   intros. induction H; assumption.
 Qed.
@@ -105,36 +108,36 @@ Qed.
 
 Ltac solve_determinism_expr expr_det :=
   match goal with
-  | [ H1 : eval_expr ?c ?G ?L ?e ?D1 ?w1 ?c1,
-      H2 : eval_expr ?c ?G ?L ?e ?D2 ?w2 ?c2 |- _ ] =>
+  | [ H1 : eval_expr ?G ?L ?e ?D1 ?w1,
+      H2 : eval_expr ?G ?L ?e ?D2 ?w2 |- _ ] =>
       let HeqD := fresh "HeqD" in
       let Heqe := fresh "Heqe" in
       let Heqc := fresh "Heqc" in
-      assert (D1 = D2 /\ w1 = w2 /\ c1 = c2) as [HeqD [Heqe Heqc]] by (eapply expr_det; eauto);
+      assert (D1 = D2 /\ w1 = w2) as [HeqD Heqe] by (eapply expr_det; eauto);
       try discriminate; try congruence; subst
   end.
 
 Ltac solve_determinism_match match_det :=
   match goal with
-  | [ H1 : eval_matching ?c ?G ?L ?A ?m ?D1 ?u1 ?c1,
-      H2 : eval_matching ?c ?G ?L ?A ?m ?D2 ?u2 ?c2 |- _ ] =>
+  | [ H1 : eval_matching ?G ?L ?A ?m ?D1 ?u1,
+      H2 : eval_matching ?G ?L ?A ?m ?D2 ?u2 |- _ ] =>
       let HeqD := fresh "HeqD" in
       let Hequ := fresh "Hequ" in
       let Heqc := fresh "Heqc" in
-      assert (D1 = D2 /\ u1 = u2 /\ c1 = c2) as [HeqD [Hequ Heqc]] by (eapply match_det; eauto);
+      assert (D1 = D2 /\ u1 = u2) as [HeqD Hequ] by (eapply match_det; eauto);
       try discriminate; try congruence; subst
   end.
 
-Lemma eval_expr_deterministic : forall c G L e D1 w1 c2 D2 w2 c3,
-  eval_expr c G L e D1 w1 c2 ->
-  eval_expr c G L e D2 w2 c3 ->
-  D1 = D2 /\ w1 = w2 /\ c2 = c3
-with eval_matching_deterministic : forall c G L A m D1 u1 c2 D2 u2 c3,
-  eval_matching c G L A m D1 u1 c2 ->
-  eval_matching c G L A m D2 u2 c3 ->
-  D1 = D2 /\ u1 = u2 /\ c2 = c3.
+Lemma eval_expr_deterministic : forall G L e D1 w1 D2 w2,
+  eval_expr G L e D1 w1 ->
+  eval_expr G L e D2 w2 ->
+  D1 = D2 /\ w1 = w2
+with eval_matching_deterministic : forall G L A m D1 u1 D2 u2,
+  eval_matching G L A m D1 u1 ->
+  eval_matching G L A m D2 u2 ->
+  D1 = D2 /\ u1 = u2.
 Proof.
-  - intros c G L e D1 w1 c2 D2 w2 c3 H1 H2.
+  - intros G L e D1 w1 D2 w2 H1 H2.
     induction H1; inversion H2; subst; try congruence.
     + auto.
     + inversion H; subst. rewrite H0 in H5. discriminate.
@@ -150,12 +153,12 @@ Proof.
       solve_determinism_expr eval_expr_deterministic.
       subst. auto.
     + inversion H0.
-    + inversion H7; subst.
+    + inversion H6; subst.
       solve_determinism_expr eval_expr_deterministic.
       inversion Heqe; subst.
       apply IHeval_expr2. assumption.
 
-  - intros c G L A m D1 u1 c2 D2 u2 c3 H1 H2.
+  - intros G L A m D1 u1 D2 u2 H1 H2.
     induction H1; inversion H2; subst; try congruence; try auto.
     + solve_determinism_expr eval_expr_deterministic.
       injection Heqe as Heqargs.
@@ -166,8 +169,10 @@ Proof.
         injection Heq. trivial.
     + solve_determinism_expr eval_expr_deterministic.
     + solve_determinism_expr eval_expr_deterministic.
-    + split; [|split]; [| trivial |]; eapply eval_expr_deterministic; eauto.
+    + split; [ | trivial ]; eapply eval_expr_deterministic; eauto.
     + solve_determinism_match eval_matching_deterministic.
     + solve_determinism_match eval_matching_deterministic.
     + solve_determinism_match eval_matching_deterministic. subst. auto.
 Qed.
+
+End FreshGen.
