theories/Big_impl_small.v
@@ -3,6 +3,9 @@ From Coq Require Import FMaps FSets.
 From Haskelite Require Import Expr Common Bigstep Smallstep.
 Import ListNotations.
 
+Section FreshGen.
+Context {FG : FreshVarGen}.
+
 Lemma whnf_lambda_arity : forall m,
   whnf (ELam m) ->
   exists n, matching_arity m = Some (S n).
@@ -12,40 +15,40 @@ Proof.
   exists n. assumption.
 Qed.
 
-Lemma eval_expr_lambda_arity : forall c G L e D m c',
-  eval_expr c G L e D (ELam m) c' ->
+Lemma eval_expr_lambda_arity : forall G L e D m,
+  eval_expr G L e D (ELam m) ->
   exists n, matching_arity m = Some (S n).
 Proof.
-  intros c G L e D m c' H.
+  intros G L e D m Hexpr.
   apply whnf_lambda_arity.
   eapply eval_expr_produces_whnf.
   eassumption.
 Qed.
 
 Theorem bigstep_impl_balancedstep :
-  (forall c G L e D w c',
-    eval_expr c G L e D w c' ->
+  (forall G L e D w,
+    eval_expr G L e D w ->
     forall St,
                L = (update_locs St) ->
                balanced_step_expr
-               {| c := c; cfg_heap := G; cfg_ctrl := CtrlExpr e; cfg_stack := St |}
-               {| c := c'; cfg_heap := D; cfg_ctrl := CtrlExpr w; cfg_stack := St |})
+               {| cfg_heap := G; cfg_ctrl := CtrlExpr e; cfg_stack := St |}
+               {| cfg_heap := D; cfg_ctrl := CtrlExpr w; cfg_stack := St |})
   /\
-  (forall c G L A m D u c',
-    eval_matching c G L A m D u c' ->
+  (forall G L A m D u,
+    eval_matching G L A m D u ->
     forall St,
                L = (update_locs St) ->
                balanced_step_matching
-               {| c := c; cfg_heap := G; cfg_ctrl := CtrlMatch A m; cfg_stack := St |}
-               {| c := c'; cfg_heap := D; cfg_ctrl := CtrlMatch []
+               {| cfg_heap := G; cfg_ctrl := CtrlMatch A m; cfg_stack := St |}
+               {| cfg_heap := D; cfg_ctrl := CtrlMatch []
                                   (match u with MRReturn e => MReturn e | MRFail => MFail end);
                   cfg_stack := St |}).
 Proof.
   apply eval_ind.
-  - intros c G L w Hwhnf St HL.
+  - intros G L w Hwhnf St HL.
     apply BExprWhnf. assumption.
 
-  - intros c c1 c2 G L m e D O w Harity Hmatch IHmatch Heval IHeval St HL.
+  - intros G L m e D O w Harity Hmatch IHmatch Heval IHeval St HL.
     eapply BExprSat.
     + exact Harity.
     + apply StepSat. exact Harity.
@@ -53,7 +56,7 @@ Proof.
     + apply StepReturn1B.
     + apply IHeval. assumption.
 
-  - intros c c1 G L y e D w Hheap Hnotin Heval IHexpr St HL.
+  - intros G L y e D w Hheap Hnotin Heval IHexpr St HL.
     eapply BExprVar.
     + exact Hheap.
     + subst L. exact Hnotin.
@@ -61,9 +64,9 @@ Proof.
     + apply IHexpr. simpl. subst L. reflexivity.
     + apply StepUpdate. eapply eval_expr_produces_whnf. eassumption.
 
-  - intros c c1 c2 G L e1 e2 m D O w x Hexpr1 IHexpr1 Hvar Hexpr2 IHexpr2 St HL.
+  - intros G L e1 e2 m D O w x Hexpr1 IHexpr1 Hvar Hexpr2 IHexpr2 St HL.
     subst e2.
-    destruct (eval_expr_lambda_arity _ _ _ _ _ _ _ Hexpr1) as [n Harity].
+    destruct (eval_expr_lambda_arity _ _ _ _ _ Hexpr1) as [n Harity].
     eapply BExprApp.
     + apply StepApp1.
     + apply IHexpr1. simpl. exact HL.
@@ -71,7 +74,7 @@ Proof.
     + apply IHexpr2. exact HL.
 
   - (* BMatchReturn *)
-    intros c G L A e St HL.
+    intros G L A e St HL.
     destruct A as [| y A'].
     + simpl. apply BMatchReturn.
     + eapply BMatchReturnArgs.
@@ -80,23 +83,23 @@ Proof.
       * apply BMatchReturn.
 
   - (* BMatchFail *)
-    intros c G L St HL.
+    intros G L St HL.
     constructor.
 
   - (* BMatchArg *)
-    intros c c' G L A x m D u Hmatch IHmatch St HL.
+    intros G L A x m D u Hmatch IHmatch St HL.
     eapply BMatchArg.
     + constructor.
     + apply IHmatch. exact HL.
 
   - (* BMatchBind *)
-    intros c c' G L A x y m D u Hmatch IHmatch St HL.
+    intros G L A x y m D u Hmatch IHmatch St HL.
     eapply BMatchBind.
     + constructor.
     + apply IHmatch. exact HL.
 
   - (* BMatchConsSuccess *)
-    intros c c1 c2 G L A x con ps m args D O u Hexpr IHexpr Hlen Hmatching IHmatching St HL.
+    intros G L A x con ps m args D O u Hexpr IHexpr Hlen Hmatching IHmatching St HL.
     eapply BMatchConsSuccess.
     + constructor.
     + apply IHexpr. simpl. exact HL.
@@ -105,7 +108,7 @@ Proof.
     + apply IHmatching. assumption.
 
   - (* BMatchConsFail *)
-    intros c c' G L A x con con' ps m args D Hexpr IHexpr Hneq St HL.
+    intros G L A x con con' ps m args D Hexpr IHexpr Hneq St HL.
     eapply BMatchConsFail.
     + exact Hneq.
     + apply StepCons1.
@@ -113,14 +116,14 @@ Proof.
     + apply StepFail. exact Hneq.
 
   - (* BMatchAltLeft *)
-    intros c c' G L A m1 m2 e D Hmatch IHmatch St HL.
+    intros G L A m1 m2 e D Hmatch IHmatch St HL.
     apply BMatchAltLeft.
     + constructor.
     + apply IHmatch. simpl. exact HL.
     + constructor.
 
   - (* BMatchAltRight *)
-    intros c c1 c2 G L A m1 m2 D O u Hmatch1 IHmatch1 Hmatch2 IHmatch2 St HL.
+    intros G L A m1 m2 D O u Hmatch1 IHmatch1 Hmatch2 IHmatch2 St HL.
     eapply BMatchAltRight.
     + constructor.
     + apply IHmatch1. simpl. exact HL.
@@ -128,24 +131,25 @@ Proof.
     + apply IHmatch2. exact HL.
 
   - (* BMatchWhere *)
-    intros c G L A m binds D u ys renamed_binds renamed_m Hys Hbinds Hm Hmatch IHmatch St HL.
+    intros G L A m binds D u ys renamed_binds renamed_m Hys Hbinds Hm Hmatch IHmatch St HL.
     eapply BMatchWhere; try eassumption.
-    + econstructor; eassumption.
-    + apply IHmatch. exact HL.
+    + subst L. assumption.
+    + econstructor; try eassumption. subst L. assumption.
+    + apply IHmatch. assumption.
 Qed.
 
 Corollary initial_bigstep_impl_balancedstep :
-  (forall e D w c',
-    eval_expr 0 empty_heap [] e D w c' ->
+  (forall e D w,
+    eval_expr empty_heap [] e D w ->
     balanced_step_expr
-      {| c := 0; cfg_heap := empty_heap; cfg_ctrl := CtrlExpr e; cfg_stack := [] |}
-      {| c := c'; cfg_heap := D; cfg_ctrl := CtrlExpr w; cfg_stack := [] |})
+      {| cfg_heap := empty_heap; cfg_ctrl := CtrlExpr e; cfg_stack := [] |}
+      {| cfg_heap := D; cfg_ctrl := CtrlExpr w; cfg_stack := [] |})
   /\
-  (forall A D m u c',
-    eval_matching 0 empty_heap [] A m D u c' ->
+  (forall A D m u,
+    eval_matching empty_heap [] A m D u ->
     balanced_step_matching
-    {| c := 0; cfg_heap := empty_heap; cfg_ctrl := CtrlMatch A m; cfg_stack := [] |}
-    {| c := c'; cfg_heap := D; cfg_ctrl := CtrlMatch []
+    {| cfg_heap := empty_heap; cfg_ctrl := CtrlMatch A m; cfg_stack := [] |}
+    {| cfg_heap := D; cfg_ctrl := CtrlMatch []
                       (match u with MRReturn e => MReturn e | MRFail => MFail end);
       cfg_stack := [] |})
 .
@@ -156,48 +160,49 @@ Proof.
 Qed.
 
 Theorem bigstep_impl_smallstep_star :
-  (forall c G L e D w c' St,
-    eval_expr c G L e D w c' ->
+  (forall G L e D w St,
+    eval_expr G L e D w ->
     L = update_locs St ->
-    {| c := c; cfg_heap := G; cfg_ctrl := CtrlExpr e; cfg_stack := St |} s=>*
-    {| c := c'; cfg_heap := D; cfg_ctrl := CtrlExpr w; cfg_stack := St |})
+    {| cfg_heap := G; cfg_ctrl := CtrlExpr e; cfg_stack := St |} s=>*
+    {| cfg_heap := D; cfg_ctrl := CtrlExpr w; cfg_stack := St |})
   /\
-  (forall c G L A m D u c' St,
-    eval_matching c G L A m D u c' ->
+  (forall G L A m D u St,
+    eval_matching G L A m D u ->
     L = update_locs St ->
-    {| c := c; cfg_heap := G; cfg_ctrl := CtrlMatch A m; cfg_stack := St |} s=>*
-    {| c := c'; cfg_heap := D; 
+    {| cfg_heap := G; cfg_ctrl := CtrlMatch A m; cfg_stack := St |} s=>*
+    {| cfg_heap := D;
        cfg_ctrl := CtrlMatch [] (match u with MRReturn e => MReturn e | MRFail => MFail end);
        cfg_stack := St |})
 .
 Proof.
   split.
-  - intros c G L e D w c' St H HL.
+  - intros G L e D w St Hexpr HL.
     apply balanced_expr_to_steps.
     apply (proj1 bigstep_impl_balancedstep) with (L := L); auto.
-  - intros c G L A m D u c' St H HL.
+  - intros G L A m D u St Hmatching HL.
     apply balanced_matching_to_steps.
     apply (proj2 bigstep_impl_balancedstep) with (L := L); auto.
 Qed.
 
 Corollary initial_bigstep_impl_smallstep :
-  (forall e D w c',
-    eval_expr 0 empty_heap [] e D w c' ->
-    {| c := 0; cfg_heap := empty_heap; cfg_ctrl := CtrlExpr e; cfg_stack := [] |} s=>*
-    {| c := c'; cfg_heap := D; cfg_ctrl := CtrlExpr w; cfg_stack := [] |})
+  (forall e D w,
+    eval_expr empty_heap [] e D w ->
+    {| cfg_heap := empty_heap; cfg_ctrl := CtrlExpr e; cfg_stack := [] |} s=>*
+    {| cfg_heap := D; cfg_ctrl := CtrlExpr w; cfg_stack := [] |})
   /\
-  (forall A D m u c',
-    eval_matching 0 empty_heap [] A m D u c' ->
-    {| c := 0; cfg_heap := empty_heap; cfg_ctrl := CtrlMatch A m; cfg_stack := [] |} s=>*
-    {| c := c'; cfg_heap := D; cfg_ctrl := CtrlMatch []
+  (forall A D m u,
+    eval_matching empty_heap [] A m D u ->
+    {| cfg_heap := empty_heap; cfg_ctrl := CtrlMatch A m; cfg_stack := [] |} s=>*
+    {| cfg_heap := D; cfg_ctrl := CtrlMatch []
                       (match u with MRReturn e => MReturn e | MRFail => MFail end);
       cfg_stack := [] |})
 .
 Proof.
   split.
-  - intros e D w c' H.
+  - intros e D w Hexpr.
     apply bigstep_impl_smallstep_star with (L := []). assumption. reflexivity.
-  - intros A D m u c' H.
+  - intros A D m u Hmatching.
     apply bigstep_impl_smallstep_star with (L := []). assumption. reflexivity.
 Qed.
 
+End FreshGen.
