theories/Small_impl_big.v
@@ -10,113 +10,112 @@ Import ListNotations.
     the LSP
 *)
 
-Lemma balanced_step_to_bigstep_expr_gen : forall c G e D w St c',
+Lemma balanced_step_to_bigstep_expr_gen {FG : FreshVarGen} : forall G e D w St,
   balanced_step_expr
-    {| c := c; cfg_heap := G; cfg_ctrl := CtrlExpr e; cfg_stack := St |}
-    {| c := c'; cfg_heap := D; cfg_ctrl := CtrlExpr w; cfg_stack := St |} ->
+    {| cfg_heap := G; cfg_ctrl := CtrlExpr e; cfg_stack := St |}
+    {| cfg_heap := D; cfg_ctrl := CtrlExpr w; cfg_stack := St |} ->
   whnf w ->
-  eval_expr c G (update_locs St) e D w c'
+  eval_expr G (update_locs St) e D w
 
-with balanced_step_to_bigstep_matching_gen : forall c G A m D A' u St c',
+with balanced_step_to_bigstep_matching_gen {FG : FreshVarGen} : forall G A m D A' u St,
   balanced_step_matching
-    {| c := c; cfg_heap := G; cfg_ctrl := CtrlMatch A m; cfg_stack := St |}
-    {| c := c'; cfg_heap := D; cfg_ctrl := CtrlMatch A' u; cfg_stack := St |} ->
+    {| cfg_heap := G; cfg_ctrl := CtrlMatch A m; cfg_stack := St |}
+    {| cfg_heap := D; cfg_ctrl := CtrlMatch A' u; cfg_stack := St |} ->
   matching_final u ->
   match u with
-  | MReturn e => eval_matching c G (update_locs St) A m D (MRReturn e) c'
-  | MFail => A' = [] /\ eval_matching c G (update_locs St) A m D MRFail c'
+  | MReturn e => eval_matching G (update_locs St) A m D (MRReturn e)
+  | MFail => A' = [] /\ eval_matching G (update_locs St) A m D MRFail
   | _ => False
   end
 .
 Proof.
-  - intros c G e D w St c' Hbal Hwhnf.
+  - intros G e D w St Hbal Hwhnf.
     inversion Hbal; subst.
     + constructor. assumption.
     + (* BExprApp *)
-      assert (Heval1 : eval_expr c G (update_locs (KArg y :: St)) e0 D0 (ELam m) c1). {
-        apply balanced_step_to_bigstep_expr_gen with (St := KArg y :: St) (c' := c1).
+      assert (Heval1 : eval_expr G (update_locs (KArg y :: St)) e0 D0 (ELam m)). {
+        apply balanced_step_to_bigstep_expr_gen with (St := KArg y :: St).
         - auto.
-        - inversion H8; subst.
+        - inversion H6; subst.
           apply whnf_lambda with n. assumption.
       }
 
-      assert (Heval2 : eval_expr c1 D0 (update_locs St) (ELam (MSupply (EVar y) m)) D w c').
-      { apply balanced_step_to_bigstep_expr_gen with (St := St) (c' := c'); assumption. }
+      assert (Heval2 : eval_expr D0 (update_locs St) (ELam (MSupply (EVar y) m)) D w).
+      { apply balanced_step_to_bigstep_expr_gen with (St := St); assumption. }
 
       simpl in Heval1.
       eapply EvalApp; eauto.
 
     + (* BExprVar *)
-      assert (Heval : eval_expr c (heap_remove G y) (update_locs (KUpdate y :: St)) e0 D0 w c').
-      { apply balanced_step_to_bigstep_expr_gen with (St := KUpdate y :: St) (c' := c'); auto. }
+      assert (Heval : eval_expr (heap_remove G y) (update_locs (KUpdate y :: St)) e0 D0 w).
+      { apply balanced_step_to_bigstep_expr_gen with (St := KUpdate y :: St); auto. }
 
       simpl in Heval. rewrite <- update_locs_KUpdate in Heval.
       eapply EvalVar; eauto.
 
     + (* BExprSat *)
-      assert (Hmatch : eval_matching c G (update_locs (KEnd :: St)) [] m D0 (MRReturn e0) c1). {
-        assert (Hmatch' := balanced_step_to_bigstep_matching_gen c G [] m D0 [] (MReturn e0) (KEnd :: St) c1 H8).
+      assert (Hmatch : eval_matching G (update_locs (KEnd :: St)) [] m D0 (MRReturn e0)). {
+        assert (Hmatch' := balanced_step_to_bigstep_matching_gen FG G [] m D0 [] (MReturn e0) (KEnd :: St) H6).
         simpl in Hmatch'. apply Hmatch'. apply MFinal_Return.
       }
 
-      assert (Heval : eval_expr c1 D0 (update_locs St) e0 D w c').
-      { apply balanced_step_to_bigstep_expr_gen with (St := St) (c' := c'); auto. }
+      assert (Heval : eval_expr D0 (update_locs St) e0 D w).
+      { apply balanced_step_to_bigstep_expr_gen with (St := St); auto. }
 
       eapply EvalSat; eauto.
 
-  - intros c G A m D A' u St c' Hbal Hfinal.
+  - intros G A m D A' u St Hbal Hfinal.
     destruct u; try (exfalso; inversion Hfinal; fail).
     + (* MReturn *)
       inversion Hbal; subst; try discriminate.
       * constructor.
       * (* BMatchReturnArgs *)
-        inversion H10; subst.
+        inversion H8; subst.
         -- apply EvalReturn.
         -- contradiction.
 
       * (* BMatchArg *)
-        assert (Heval : eval_matching c G (update_locs St) (y :: A) m0 D (MRReturn e) c').
+        assert (Heval : eval_matching G (update_locs St) (y :: A) m0 D (MRReturn e)).
         { apply balanced_step_to_bigstep_matching_gen with (A' := A') (u := MReturn e); auto. }
         eapply EvalArg. eauto.
 
       * (* BMatchBind *)
-        assert (Heval : eval_matching c G (update_locs St) A0 (subst_matching m0 y x) D (MRReturn e) c').
+        assert (Heval : eval_matching G (update_locs St) A0 (subst_matching m0 y x) D (MRReturn e)).
         { apply balanced_step_to_bigstep_matching_gen with (A' := A') (u := MReturn e); auto. }
         eapply EvalBindVar. eauto.
 
       * (* BMatchConsSuccess *)
-        assert (Heval_expr : eval_expr c G (update_locs (KPat A0 cp ps m0 :: St)) (EVar x) D0 (ECons cp (map EVar args)) c1).
+        assert (Heval_expr : eval_expr G (update_locs (KPat A0 cp ps m0 :: St)) (EVar x) D0 (ECons cp (map EVar args))).
         { apply balanced_step_to_bigstep_expr_gen; auto. constructor. }
 
-        assert (Heval_match : eval_matching c1 D0 (update_locs St) A0 (build_nested_matches args ps m0) D (MRReturn e) c').
+        assert (Heval_match : eval_matching D0 (update_locs St) A0 (build_nested_matches args ps m0) D (MRReturn e)).
         { apply balanced_step_to_bigstep_matching_gen with (A' := A') (u := MReturn e); auto. }
 
         eapply EvalConsMatch; eauto.
 
       * (* BMatchAltLeft *)
-        assert (Heval : eval_matching c G (update_locs (KAlt A m2 :: St)) A m1 D (MRReturn e) c').
+        assert (Heval : eval_matching G (update_locs (KAlt A m2 :: St)) A m1 D (MRReturn e)).
         { apply balanced_step_to_bigstep_matching_gen with (A' := []) (u := MReturn e); auto. }
         simpl in Heval.
         eapply EvalAltLeft. eassumption.
 
       * (* BMatchAltRight *)
-        assert (Hm1 := balanced_step_to_bigstep_matching_gen _ _ _ _ _ _ _ _ _ H9 MFinal_Fail).
+        assert (Hm1 := balanced_step_to_bigstep_matching_gen FG _ _ _ _ _ _ _ H7 MFinal_Fail).
         destruct Hm1 as [_ Hm1].
 
-        assert (Hm2: eval_matching c1 D0 (update_locs St) A m2 D (MRReturn e) c').
+        assert (Hm2: eval_matching D0 (update_locs St) A m2 D (MRReturn e)).
         { apply balanced_step_to_bigstep_matching_gen with (A' := A') (u := MReturn e); auto. }
 
         eapply EvalAltRight; eauto.
 
       * (* BMatchWhere *)
-        set (renamed_binds := rename_bindings binds (gen_n_fresh c (Datatypes.length binds))).
-        set (renamed_m := rename_matching m0 (gen_n_fresh c (Datatypes.length binds)) binds).
+        set (renamed_binds := rename_bindings binds (gen_fresh (update_locs St) (Datatypes.length binds))).
+        set (renamed_m := rename_matching m0 (gen_fresh (update_locs St) (Datatypes.length binds)) binds).
         assert (Heval :
-          eval_matching (c + length binds) (allocate_bindings G renamed_binds) (update_locs St) A renamed_m
-          D (MRReturn e) (c + length binds)).
+          eval_matching (allocate_bindings G renamed_binds) (update_locs St) A renamed_m D (MRReturn e)).
         {
-          apply (balanced_step_to_bigstep_matching_gen (c + length binds) (allocate_bindings G renamed_binds) A renamed_m
-                 D A' (MReturn e) St (c + length binds)); auto.
+          apply (balanced_step_to_bigstep_matching_gen FG (allocate_bindings G renamed_binds) A renamed_m
+                 D A' (MReturn e) St); auto.
         }
 
         eapply EvalWhere; eauto.
@@ -128,14 +127,14 @@ Proof.
         constructor.
 
       * (* BMatchArg *)
-        assert (Hinner_result : A' = [] /\ eval_matching c G (update_locs St) (y :: A) m0 D MRFail c').
+        assert (Hinner_result : A' = [] /\ eval_matching G (update_locs St) (y :: A) m0 D MRFail).
         { apply balanced_step_to_bigstep_matching_gen with (A' := A') (u := MFail); auto. }
         destruct Hinner_result as [HA' Hinner_eval].
         split; [ assumption | ].
         eapply EvalArg. eassumption.
 
       * (* BMatchBind *)
-        assert (Hsubst_result : A' = [] /\ eval_matching c G (update_locs St) A0 (subst_matching m0 y x) D MRFail c').
+        assert (Hsubst_result : A' = [] /\ eval_matching G (update_locs St) A0 (subst_matching m0 y x) D MRFail).
         { apply balanced_step_to_bigstep_matching_gen with (A' := A') (u := MFail); auto. }
         destruct Hsubst_result as [HA' Hsubst_eval].
 
@@ -143,10 +142,10 @@ Proof.
         eapply EvalBindVar. eassumption.
 
       * (* BMatchConsSuccess *)
-        assert (Hnested_result : A' = [] /\ eval_matching c1 D0 (update_locs St) A0 (build_nested_matches args ps m0) D MRFail c').
+        assert (Hnested_result : A' = [] /\ eval_matching D0 (update_locs St) A0 (build_nested_matches args ps m0) D MRFail).
         { apply balanced_step_to_bigstep_matching_gen with (A' := A') (u := MFail); auto. }
         destruct Hnested_result as [HA' Hnested_eval].
-        assert (Hexpr : eval_expr c G (update_locs (KPat A0 cp ps m0 :: St)) (EVar x) D0 (ECons cp (map EVar args)) c1).
+        assert (Hexpr : eval_expr G (update_locs (KPat A0 cp ps m0 :: St)) (EVar x) D0 (ECons cp (map EVar args))).
         { apply balanced_step_to_bigstep_expr_gen with (w := ECons cp (map EVar args)); auto. constructor. }
 
         split; [ assumption | ].
@@ -154,7 +153,7 @@ Proof.
         eapply EvalConsMatch; eauto.
 
       * (* BMatchConsFail *)
-        assert (Hexpr : eval_expr c G (update_locs (KPat A0 cp ps m0 :: St)) (EVar x) D (ECons cp' args) c').
+        assert (Hexpr : eval_expr G (update_locs (KPat A0 cp ps m0 :: St)) (EVar x) D (ECons cp' args)).
         { apply balanced_step_to_bigstep_expr_gen with (w := ECons cp' args); auto. constructor. }
 
         split; [ reflexivity | ].
@@ -162,11 +161,11 @@ Proof.
         eapply EvalConsFail; eauto.
 
       * (* BMatchAltRight fail *)
-        assert (Hm1 : @nil var = [] /\ eval_matching c G (update_locs (KAlt A m2 :: St)) A m1 D0 MRFail c1).
+        assert (Hm1 : @nil var = [] /\ eval_matching G (update_locs (KAlt A m2 :: St)) A m1 D0 MRFail).
         { apply balanced_step_to_bigstep_matching_gen with (A' := []) (u := MFail); auto. }
         destruct Hm1 as [_ Hm1].
 
-        assert (Hm2 : A' = [] /\ eval_matching c1 D0 (update_locs St) A m2 D MRFail c').
+        assert (Hm2 : A' = [] /\ eval_matching D0 (update_locs St) A m2 D MRFail).
         { apply balanced_step_to_bigstep_matching_gen with (A' := A') (u := MFail); auto. }
         destruct Hm2 as [HA' Hm2].
 
@@ -175,22 +174,21 @@ Proof.
         eapply EvalAltRight; eauto.
 
       * (* BMatchWhere *)
-        assert (HFail : A' = [] /\ eval_matching (c + Datatypes.length binds)
+        assert (HFail : A' = [] /\ eval_matching
                                     (allocate_bindings G
-                                    (rename_bindings binds (gen_n_fresh c (Datatypes.length binds))))
+                                    (rename_bindings binds (gen_fresh (update_locs St) (Datatypes.length binds))))
                                     (update_locs St) A
-                                    (rename_matching m0 (gen_n_fresh c (Datatypes.length binds)) binds)
-                                    D MRFail (c + Datatypes.length binds)).
+                                    (rename_matching m0 (gen_fresh (update_locs St) (Datatypes.length binds)) binds)
+                                    D MRFail).
         {
-          apply (balanced_step_to_bigstep_matching_gen
-                   (c + Datatypes.length binds)
-                   (allocate_bindings G (rename_bindings binds (gen_n_fresh c (Datatypes.length binds))))
+          apply (balanced_step_to_bigstep_matching_gen FG
+                   (allocate_bindings G (rename_bindings binds (gen_fresh (update_locs St) (Datatypes.length binds))))
                    A
-                   (rename_matching m0 (gen_n_fresh c (Datatypes.length binds)) binds)
-                   D A' MFail St (c + Datatypes.length binds));
+                   (rename_matching m0 (gen_fresh (update_locs St) (Datatypes.length binds)) binds)
+                   D A' MFail St);
           auto.
         }
         destruct HFail as [HA HEval].
         split; auto.
-        eapply EvalWhere with (ys := gen_n_fresh c (Datatypes.length binds)); eauto.
+        eapply EvalWhere with (ys := gen_fresh (update_locs St) (Datatypes.length binds)); eauto.
 Qed.
